program_logic/ectx_lifting.v
@@ -39,19 +39,17 @@ Proof.
 Qed.
 
 Lemma wp_lift_atomic_head_step {E Φ} e1 σ1 :
-  atomic e1 →
   head_reducible e1 σ1 →
-  ▷ ownP σ1 ∗ ▷ (∀ v2 σ2 efs,
-  ⌜head_step e1 σ1 (of_val v2) σ2 efs⌝ ∧ ownP σ2 -∗
-    Φ v2 ∗ [∗ list] ef ∈ efs, WP ef {{ _, True }})
+  ▷ ownP σ1 ∗ ▷ (∀ e2 σ2 efs,
+  ⌜head_step e1 σ1 e2 σ2 efs⌝ ∧ ownP σ2 -∗
+    default False (to_val e2) Φ ∗ [∗ list] ef ∈ efs, WP ef {{ _, True }})
   ⊢ WP e1 @ E {{ Φ }}.
 Proof.
-  iIntros (??) "[? H]". iApply wp_lift_atomic_step; eauto. iFrame. iNext.
+  iIntros (?) "[? H]". iApply wp_lift_atomic_step; eauto. iFrame. iNext.
   iIntros (???) "[% ?]". iApply "H". eauto.
 Qed.
 
 Lemma wp_lift_atomic_det_head_step {E Φ e1} σ1 v2 σ2 efs :
-  atomic e1 →
   head_reducible e1 σ1 →
   (∀ e2' σ2' efs', head_step e1 σ1 e2' σ2' efs' →
     σ2 = σ2' ∧ to_val e2' = Some v2 ∧ efs = efs') →
@@ -61,7 +59,6 @@ Lemma wp_lift_atomic_det_head_step {E Φ e1} σ1 v2 σ2 efs :
 Proof. eauto using wp_lift_atomic_det_step. Qed.
 
 Lemma wp_lift_atomic_det_head_step' {E e1} σ1 v2 σ2 :
-  atomic e1 →
   head_reducible e1 σ1 →
   (∀ e2' σ2' efs', head_step e1 σ1 e2' σ2' efs' →
     σ2 = σ2' ∧ to_val e2' = Some v2 ∧ [] = efs') →
