program_logic/lifting.v
@@ -45,23 +45,21 @@ Qed.
 
 (** Derived lifting lemmas. *)
 Lemma wp_lift_atomic_step {E Φ} e1 σ1 :
-  atomic e1 →
   reducible e1 σ1 →
-  (▷ ownP σ1 ∗ ▷ ∀ v2 σ2 efs, ⌜prim_step e1 σ1 (of_val v2) σ2 efs⌝ ∗ ownP σ2 -∗
-    Φ v2 ∗ [∗ list] ef ∈ efs, WP ef {{ _, True }})
+  (▷ ownP σ1 ∗ ▷ ∀ e2 σ2 efs, ⌜prim_step e1 σ1 e2 σ2 efs⌝ ∗ ownP σ2 -∗
+    default False (to_val e2) Φ ∗ [∗ list] ef ∈ efs, WP ef {{ _, True }})
   ⊢ WP e1 @ E {{ Φ }}.
 Proof.
-  iIntros (Hatomic ?) "[Hσ H]". iApply (wp_lift_step E _ e1).
+  iIntros (?) "[Hσ H]". iApply (wp_lift_step E _ e1).
   iMod (fupd_intro_mask' E ∅) as "Hclose"; first set_solver. iModIntro.
   iExists σ1. iFrame "Hσ"; iSplit; eauto.
   iNext; iIntros (e2 σ2 efs) "[% Hσ]".
-  edestruct (Hatomic σ1 e2 σ2 efs) as [v2 <-%of_to_val]; eauto.
-  iDestruct ("H" $! v2 σ2 efs with "[Hσ]") as "[HΦ $]"; first by eauto.
-  iMod "Hclose". iApply wp_value; auto using to_of_val.
+  iDestruct ("H" $! e2 σ2 efs with "[Hσ]") as "[HΦ $]"; first by eauto.
+  destruct (to_val e2) eqn:?; last by iExFalso.
+  iMod "Hclose". iApply wp_value; auto using to_of_val. done.
 Qed.
 
 Lemma wp_lift_atomic_det_step {E Φ e1} σ1 v2 σ2 efs :
-  atomic e1 →
   reducible e1 σ1 →
   (∀ e2' σ2' efs', prim_step e1 σ1 e2' σ2' efs' →
                    σ2 = σ2' ∧ to_val e2' = Some v2 ∧ efs = efs') →
@@ -69,9 +67,9 @@ Lemma wp_lift_atomic_det_step {E Φ e1} σ1 v2 σ2 efs :
     Φ v2 ∗ [∗ list] ef ∈ efs, WP ef {{ _, True }})
   ⊢ WP e1 @ E {{ Φ }}.
 Proof.
-  iIntros (?? Hdet) "[Hσ1 Hσ2]". iApply (wp_lift_atomic_step _ σ1); try done.
-  iFrame. iNext. iIntros (v2' σ2' efs') "[% Hσ2']".
-  edestruct Hdet as (->&->%of_to_val%(inj of_val)&->). done. by iApply "Hσ2".
+  iIntros (? Hdet) "[Hσ1 Hσ2]". iApply (wp_lift_atomic_step _ σ1); try done.
+  iFrame. iNext. iIntros (e2' σ2' efs') "[% Hσ2']".
+  edestruct Hdet as (->&Hval&->). done. rewrite Hval. by iApply "Hσ2".
 Qed.
 
 Lemma wp_lift_pure_det_step `{Inhabited (state Λ)} {E Φ} e1 e2 efs :
